src/lowparse/LowParse.Low.Base.fst
@@ -120,7 +120,7 @@ let accessor_compose
   (#t3: Type)
   (#p3: parser k3 t3)
   (#cl23: clens t2 t3)
-  (#a23: gaccessor p2 p3 cl23 { k2.parser_kind_subkind == Some ParserStrong })
+  (#a23: gaccessor p2 p3 cl23 { k2.parser_kind_injective == true })
   (a23' : accessor a23)
 : Tot (accessor (gaccessor_compose a12 a23))
 = fun #rrel #rel input pos ->
