src/lowparse/LowParse.Low.IfThenElse.fst
@@ -248,6 +248,7 @@ let gaccessor_ifthenelse_payload
   (b: bool)
 : Tot (gaccessor (parse_ifthenelse p) (dsnd (p.parse_ifthenelse_payload_parser b)) (clens_ifthenelse_payload s b))
 = Classical.forall_intro_2 (fun x -> Classical.move_requires (gaccessor_ifthenelse_payload_no_lookahead s b x));
+  Classical.forall_intro_2 (fun x -> Classical.move_requires (gaccessor_ifthenelse_payload_injective s b x));
   gaccessor_prop_equiv (parse_ifthenelse p) (dsnd (p.parse_ifthenelse_payload_parser b)) (clens_ifthenelse_payload s b) (gaccessor_ifthenelse_payload' s b);
   gaccessor_ifthenelse_payload' s b
 
